coq/theories/Examples/IPv4.v
@@ -4,21 +4,21 @@ Open Scope string_scope.
 
 Definition meta_t : typ :=
   (* drop flag, port number *)
-  Prod [Bool; Bit 8].
+  Prod Bool (Bit 8).
 
 Definition ipv4_t : typ :=
   (* src addr, dst addr *)
-  Prod [Bit 8; Bit 8].
+  Prod (Bit 8) (Bit 8).
 
 Definition zeros (n: nat) : exp :=
   Bits (List.repeat false n).
 
 Definition set_out : action :=
-  ActAssign "meta" (Tuple [EBool false; (Proj (Var "ip") 1)]).
+  ActAssign "meta" (Tuple (EBool false) (Proj1 (Var "ip"))).
 
 Definition ipv4_defns : list defn :=
-  [VarDecl ipv4_t "ip" (Tuple [zeros 8; zeros 8]);
-   Table "route" (Proj (Var "ip") 1) [set_out]].
+  [VarDecl ipv4_t "ip" (Tuple (zeros 8) (zeros 8));
+   Table "route" (Proj1 (Var "ip")) [set_out]].
 
 Definition ipv4_cmd : cmd :=
   Seq (Extr "ip")
