coq/theories/LivenessProof.v
@@ -165,7 +165,208 @@ Proof.
   intro; subst; tauto.
 Qed.
 
-Lemma dse_corr:
+Lemma agree_trans:
+  forall live x y z,
+    agree live x y ->
+    agree live y z ->
+    agree live x z.
+Proof.
+  unfold agree.
+  intros live x y z.
+  rewrite !Forall_forall.
+  intros.
+  erewrite H; eauto.
+Qed.
+
+Lemma agree_sym:
+  forall live x y,
+    agree live x y ->
+    agree live y x.
+Proof.
+  unfold agree.
+  intros live x y.
+  rewrite !Forall_forall.
+  firstorder.
+Qed.
+
+Lemma agree_assign_dead:
+  forall live s1 s2 x v,
+    check x live = false ->
+    agree live (store s1) (store s2) ->
+    agree live (store (assign s1 x v)) (store (assign s2 x v)).
+Proof.
+  simpl.
+  intros.
+  eapply agree_trans.
+  apply agree_bind_neq; auto.
+  apply agree_sym.
+  eapply agree_trans.
+  apply agree_bind_neq; auto.
+  apply agree_sym.
+  apply H0.
+Qed.
+
+Lemma check_in:
+  forall x s,
+    check x s = true <-> In x s.
+Proof.
+  unfold check.
+  intros x s.
+  destruct (in_dec _ x s); intuition.
+Qed.
+
+Lemma agree_find:
+  forall x live s1 s2,
+    check x live = true ->
+    agree live s1 s2 ->
+    Env.find x s1 = Env.find x s2.
+Proof.
+  unfold agree.
+  intros.
+  rewrite Forall_forall in H0.
+  eapply H0.
+  apply check_in.
+  auto.
+Qed.
+
+Lemma agree_emp:
+  forall s1 s2,
+    agree emp s1 s2.
+Proof.
+  intros.
+  apply Forall_nil.
+Qed.
+
+Lemma agree_cons:
+  forall a s e1 e2,
+    Env.find a e1 = Env.find a e2 ->
+    agree s e1 e2 ->
+    agree (a :: s) e1 e2.
+Proof.
+  intros.
+  apply Forall_cons; eauto.
+Qed.
+
+Lemma agree_union:
+  forall s2 s1 e1 e2,
+    agree (union s1 s2) e1 e2 ->
+    agree s1 e1 e2 /\ 
+    agree s2 e1 e2.
+Proof.
+  induction s2; simpl; intros.
+  - eauto using agree_emp.
+  - unfold add in H.
+    destruct (check a s1) eqn:?.
+    + apply IHs2 in H.
+      intuition.
+      eapply agree_cons; eauto.
+      eapply Forall_forall in H0; eauto.
+      eapply check_in; eauto.
+    + apply IHs2 in H.
+      intuition.
+      * eapply Forall_forall.
+        intros.
+        eapply Forall_forall in H0.
+        eapply H0.
+        eauto with datatypes.
+      * eapply agree_cons; eauto.
+        eapply Forall_forall in H0; eauto.
+        simpl; tauto.
+Qed.
+
+Lemma agree_union_l:
+  forall s1 s2 e1 e2,
+    agree (union s1 s2) e1 e2 ->
+    agree s1 e1 e2.
+Proof.
+  intros.
+  apply agree_union in H.
+  tauto.
+Qed.
+
+Lemma agree_union_r:
+  forall s1 s2 e1 e2,
+    agree (union s1 s2) e1 e2 ->
+    agree s2 e1 e2.
+Proof.
+  intros.
+  apply agree_union in H.
+  tauto.
+Qed.
+
+Lemma dse_exp_corr:
+  forall s s' e,
+    agree (fv e) s.(store) s'.(store) ->
+    interp_exp s e = interp_exp s' e.
+Proof.
+  induction e; simpl; intros.
+  - eapply agree_find; eauto.
+    apply check_cons_eq.
+  - reflexivity.
+  - reflexivity.
+  - apply agree_union in H; destruct H.
+    rewrite IHe1 by eauto.
+    rewrite IHe2 by eauto.
+    reflexivity.
+  - reflexivity.
+  - rewrite IHe by eauto.
+    reflexivity.
+  - rewrite IHe by eauto.
+    reflexivity.
+  - apply agree_union in H; destruct H.
+    rewrite IHe1 by eauto.
+    rewrite IHe2 by eauto.
+    reflexivity.
+  - rewrite IHe by eauto.
+    reflexivity.
+Qed.
+
+Lemma pkt_assign:
+  forall s x v,
+    pkt (assign s x v) = pkt s.
+Proof.
+  reflexivity.
+Qed.
+
+Lemma in_drop_neq:
+  forall x y s,
+    x <> y ->
+    In x s ->
+    In x (drop y s).
+Proof.
+  intros.
+  unfold drop.
+  apply in_in_remove; eauto.
+Qed.
+
+Lemma agree_bind:
+  forall x live v s1 s2,
+    agree (drop x live) s1 s2 ->
+    agree live (Env.bind x v s1) (Env.bind x v s2).
+Proof.
+  intros.
+  apply Forall_forall; intros.
+  destruct (name_eq_dec x x0).
+  - cbv in e.
+    subst x0.
+    rewrite !Env.find_bind_eq.
+    reflexivity.
+  - rewrite !Env.find_bind_neq by auto.
+    eapply Forall_forall in H; eauto.
+    apply in_drop_neq; eauto.
+Qed.
+
+Lemma agree_assign:
+  forall live s1 s2 x v,
+    agree (drop x live) (store s1) (store s2) ->
+    agree live (store (assign s1 x v)) (store (assign s2 x v)).
+Proof.
+  simpl.
+  intros.
+  apply agree_bind; auto.
+Qed.
+
+Lemma dse_cmd_corr:
   forall c live live' c' ds,
     dead_store_elim ds.(tables) live c = (live', c') ->
     forall n s1 s1',
@@ -180,11 +381,32 @@ Lemma dse_corr:
 Proof.
   induction c; simpl; intros.
   - destruct n; simpl in * |-; try congruence.
+    destruct (interp_exp s1 e) eqn:?; simpl in * |-; try congruence.
     destruct (check x live) eqn:?; inversion H; clear H; subst.
     + simpl.
-      admit.
-    + admit.
-  - admit.
+      inversion H0; subst.
+      pose proof (agree_union_r _ _ _ _ H1).
+      apply dse_exp_corr in H.
+      rewrite Heqo in *.
+      rewrite H in *.
+      destruct (interp_exp s2 e) eqn:?; simpl in *; try congruence.
+      exists (assign s2 x v).
+      erewrite !pkt_assign in *; eauto.
+      inversion H.
+      intuition.
+      apply agree_assign.
+      eapply agree_union_l; eauto.
+    + exists s2.
+      inversion H0; subst.
+      clear H0.
+      simpl; intuition.
+      * eapply agree_trans.
+        apply agree_bind_neq; eauto.
+        eauto.
+  - inversion H; subst.
+    exists s2.
+    destruct n; simpl in *; try congruence.
+    intuition congruence.
   - destruct n; try solve [simpl in H0; congruence].
     simpl in H0.
     destruct (interp_cmd n ds s1 c1) eqn:?;
